\documentclass{article}
\usepackage{amsmath}

\begin{document}

\section*{Difference Formula}

Given:
\begin{itemize}
    \item \( x \) is the primary integer
    \item \( i \) is the iterator
\end{itemize}

The two answers are:
\[
\text{primeAnsweragen} = x \cdot i
\]
\[
\text{secondaryAnsweragen} = (x - 1) \cdot (i + 1)
\]

The difference between \text{primeAnsweragen} and \text{secondaryAnsweragen} is:
\[
\text{difference} = (x \cdot i) - [(x - 1) \cdot (i + 1)]
\]

Expanding and simplifying:
\[
\text{difference} = x \cdot i - (x - 1) \cdot (i + 1)
\]
\[
\text{difference} = x \cdot i - (x \cdot i + x - i - 1)
\]
\[
\text{difference} = x \cdot i - x \cdot i - x + i + 1
\]
\[
\text{difference} = -x + i + 1
\]

So, the formula for the difference is:
\[
\text{difference} = i - x + 1
\]

\section*{Ratio Formula}

The ratio of \text{secondaryAnsweragen} to \text{primeAnsweragen} is:
\[
\text{ratio} = \frac{(x - 1) \cdot (i + 1)}{x \cdot i}
\]

Expanding and simplifying:
\[
\text{ratio} = \frac{(x - 1) \cdot (i + 1)}{x \cdot i}
\]
\[
\text{ratio} = \frac{(x - 1) \cdot i + (x - 1)}{x \cdot i}
\]
\[
\text{ratio} = \frac{(x - 1) \cdot i}{x \cdot i} + \frac{x - 1}{x \cdot i}
\]
\[
\text{ratio} = \frac{x - 1}{x} + \frac{x - 1}{x \cdot i}
\]
\[
\text{ratio} = 1 - \frac{1}{x} + \frac{x - 1}{x \cdot i}
\]

So, the formula for the ratio is:
\[
\text{ratio} = 1 - \frac{1}{x} + \frac{x - 1}{x \cdot i}
\]

These LaTeX formulas describe the relationship between the difference and the ratio of the two answers generated by your algorithm.

\end{document}